Adequacy statements

theories/program_logic/delayfreewp.v
@@ -2,7 +2,7 @@ From stdpp Require Import base gmap.
 From iris.algebra Require Import auth gmap excl.
 From iris.proofmode Require Import base tactics classes.
 From iris.base_logic.lib Require Export fancy_updates.
-From shiris.program_logic Require Import delayfree.
+From shiris.program_logic Require Import delayfree evaluation.
 Set Default Proof Using "Type".
 
 (* Curry the value R so it can be changed by the dependent pattern match on c *)
@@ -21,10 +21,10 @@ Definition wp_pre {Σ} {V} (SI: gmap loc V -> iProp Σ)
      discrete_funO (λ R, expr V R -d> (R -d> iPropO Σ) -d> iPropO Σ).
 refine(λ R e Φ,
         match e with
-        |Answer x => Φ x 
-        |Think e' => ▷ go R e' Φ
-        |Fork e' k => ▷ (go R k Φ ∗ go unit e' (λ _, True))
-        |Vis c k => ∀σ, SI σ ==∗ ∃σ' v, ⌜command_predicate c σ σ' v⌝ ∗ SI σ' ∗ ▷ (go R (k v)) Φ
+        |Answer x  => |==> Φ x 
+        |Think e'  => |==> ▷ go R e' Φ
+        |Fork e' k => |==> ▷ (go R k Φ ∗ go unit e' (λ _, True))
+        |Vis c k   => ∀σ, SI σ ==∗ ▷ |==> ∃σ' v, ⌜command_predicate c σ σ' v⌝ ∗ SI σ' ∗ (go R (k v)) Φ
         end
 )%I.
 Defined.
@@ -41,6 +41,16 @@ Definition wp' {Σ} {V} (SI: gmap nat V -> iProp Σ)
 
 Definition wp {Σ} {V R} (SI: gmap nat V -> iProp Σ) (e: expr V R) (Φ: R -> iProp Σ): iProp Σ := 
     wp' SI R e Φ.
+
+Definition wp_thread {Σ} {V R} (SI: gmap nat V -> iProp Σ) (t: thread V R) 
+: (R -> iProp Σ) -> iProp Σ.
+refine (
+  match t with
+  | Main e => wp SI e
+  | Forked e => λ _,  wp SI e (λ _, True)
+  end
+)%I.
+Defined.
 
 Lemma wp_unfold {Σ} {V R} (e: expr V R) (SI: gmap nat V -> iProp Σ) (Φ: R -> iProp Σ)
   : wp SI e Φ ≡  wp_pre SI (wp' SI) R e Φ.
@@ -74,22 +84,23 @@ Proof.
   unfold wp_pre.
   destruct e; simpl.
   - do 2 (rewrite wp_unfold /=). unfold wp_pre.
-    done.
+    by destruct (f r); iMod "H".
   - iEval (rewrite wp_unfold /=) in "H".
-    iNext. iApply "IH". done.
+    iMod "H". iIntros "!> !>". iApply "IH". done.
   - iEval (rewrite wp_unfold /=) in "H".
-    iNext. iDestruct "H" as "(H & $)". 
+     iMod "H" as "(H & $)". iIntros "!> !>". 
     iApply "IH". done.
   - iIntros (σ)  "HSi".
     iEval (rewrite wp_unfold /=) in "H".
     iMod ("H" $! σ with "HSi") as "H". iModIntro.
-    iDestruct ("H") as (σ' v) "H".
+    iNext.
+    iMod ("H") as (σ' v) "H". iModIntro.
     iExists σ', v.
     iDestruct "H" as  "($ & $ & Hwp)". 
-    iNext. iApply "IH". done.
+    iApply "IH". done.
 Qed.
 
-Lemma wp_mono {Σ} {V R: Type} (SI: gmap nat V -> iProp Σ)
+(* Lemma wp_mono {Σ} {V R: Type} (SI: gmap nat V -> iProp Σ)
    (e: expr V R) (Φ Ψ: R -> iProp Σ)
    :wp SI e Φ -∗ (∀ v, Φ v -∗ Ψ v) -∗ wp SI e Ψ.
 Proof.
@@ -108,7 +119,7 @@ Proof.
     iDestruct "Hwp'" as (σ' v) "(Hcom & HSi' & Hwp'')".
     iModIntro. iExists σ', v. iFrame. iNext.
     iApply ("IH"  with "Hwp'' H"). 
-  Qed.
+  Qed. *)
 
 (* 
   This is currently not provable because there is no update modality
@@ -124,36 +135,180 @@ Proof.
   rewrite wp_unfold.
   iIntros "Hwp H".
   destruct e; simpl.
-  - iDestruct ("H" with "Hwp") as "bla".
-    admit.
-    (* iMod "Hwp" as "Hwp". iApply ("H" with "Hwp"). *)
+  - iMod ("H" with "Hwp").
+    done.
+  - iMod "Hwp". iIntros "!> !>". 
+    iApply ("IH" $! e with "Hwp H").
   - admit.
-    (* iMod "Hwp" as "Hwp". iModIntro. *)
-    (* iNext. iApply ("IH" $! e with "Hwp H").  *)
+  - iIntros (σ) "HSi".
+    iMod ("Hwp" with "HSi") as "Hwp".
+    iIntros "!> !>".
+    iMod "Hwp". iModIntro.
+    iDestruct "Hwp" as (σ' v) "(Hcom & HSi & Hwp)".
+    iExists σ', v. iFrame. 
+    iApply ("IH"  with "Hwp H"). 
 Admitted.
 
-Lemma wp_delay_fmap {Σ} {V R B: Type} (SI: gmap nat V -> iProp Σ) 
-  (f: R -> B) (Φ: B -> iProp Σ) (e: expr V R)
-  : wp SI e (Φ ∘ f ) -∗ wp SI (f <$> e) Φ. 
+(* Lemma wp_delay_fmap {Σ} {V R B: Type} (SI: gmap nat V -> iProp Σ)  *)
+  (* (f: R -> B) (Φ: B -> iProp Σ) (e: expr V R) *)
+  (* : wp SI e (Φ ∘ f ) -∗ wp SI (f <$> e) Φ.  *)
+(* Proof. *)
+  (* iIntros "Hwp". *)
+  (* iApply wp_bind. *)
+  (* iApply (wp_mono with "Hwp"). *)
+  (* iIntros (x) "Hpost /=". *)
+  (* iApply (wp_return with "Hpost"). *)
+(* Qed. *)
+(*  *)
+(* Lemma wp_delay_iter {Σ} {V R B: Type} (SI: gmap nat V -> iProp Σ) (Φ: B -> iProp Σ) *)
+  (* (x: R) *)
+  (* (f: R -> expr V (R + B)): *)
+  (* wp SI (f x) (case_ (λ x, ▷ wp SI (iter f x) Φ) Φ) -∗ *)
+  (* wp SI (iter f x) Φ. *)
+(* Proof. *)
+  (* iIntros "Hwp". *)
+  (* rewrite iter_unfold. *)
+  (* iApply wp_bind. *)
+  (* iApply (wp_mono with "Hwp"). *)
+  (* iIntros ([a | b]) "H /=". *)
+  (* - by iApply wp_think. *)
+  (* - by iApply wp_return. *)
+(* Qed. *)
+
+(* Lemma adequacy_state_delay {A} (φ: A -> Prop) (n: nat) (x: A)  *)
+  (* (prog : state_delay (gmap nat nat) A) *)
+  (* (st st': gmap nat nat) *)
+  (* : (∀γ, ⊢ wp (state_interp γ) prog (λ x, ⌜φ x⌝)) -> *)
+  (* eval_state_delay' n prog st = Some (st', x) -> *)
+  (* φ x.  *)
+(* maak thread indexing een progerr zodat adequacy dat uitsluit *)
+(*Heap rules *)
+Definition heapR (A: ofeT): cmraT := authR (gmapUR nat (exclR A)).
+
+Lemma fresh_none (σ: gmap nat nat): 
+  let l := fresh (dom (gset nat) σ)
+  in σ !! l = None.
 Proof.
-  iIntros "Hwp".
-  iApply wp_bind.
-  iApply (wp_mono with "Hwp").
-  iIntros (x) "Hpost /=".
-  iApply (wp_return with "Hpost").
+  apply (not_elem_of_dom (D := gset nat)).
+  apply is_fresh.
 Qed.
 
-Lemma wp_delay_iter {Σ} {V R B: Type} (SI: gmap nat V -> iProp Σ) (Φ: B -> iProp Σ)
-  (x: R)
-  (f: R -> expr V (R + B)):
-  wp SI (f x) (case_ (λ x, ▷ wp SI (iter f x) Φ) Φ) -∗
-  wp SI (iter f x) Φ.
+
+Section adequacy.
+Context `{! inG Σ (heapR natO)}.
+
+(* Now come the rule that needs the points to connective in their weakest pre definition.
+    We therefore first define this in terms of the Authorative camera.
+  *)
+
+ Definition points_to (γ: gname) (n: nat) (v: nat): iProp Σ :=
+   own γ ( ◯ {[ n := Excl v ]}).
+
+ Definition lift_excl (σ: gmap nat nat): (gmap nat (excl nat)) := (Excl <$> σ).
+ Definition state_interp (γ: gname) (σ: gmap nat nat) := own γ (● (lift_excl σ)).
+ Context (γ: gname).
+
+(*
+
+
+Definition step_expr {V R A} (e: expr V A): state V R (expr V A) :=
+Definition step_thread {V R} (t: thread V R) : state V R (thread V R) :=
+Definition single_step_thread {V R} (s: scheduler V R): state V R (scheduler V R ) :=
+Fixpoint eval_threaded {V R} (n: nat) (s : scheduler V R) {struct n}: state V R R :=
+*)
+Lemma step_expr_adequacy {R A} (Φ: R -> iProp Σ) (Ψ: A -> iProp Σ) 
+  (h: heap nat)
+  (ts: list (thread nat R))
+  (e: expr nat A):
+  wp (state_interp γ) e Ψ -∗
+  state_interp γ h -∗
+  ([∗ list] t ∈ ts, wp_thread (state_interp γ) t Φ) ==∗ ▷
+  match runState (step_expr e) h ts with
+  | Here (e', h', ts') => wp (state_interp γ) e' Ψ ∗ state_interp γ h'
+                          ∗ [∗ list] t ∈ ts', wp_thread (state_interp γ) t Φ
+  | ProgErr => False
+  | EvalErr => True
+  end.
 Proof.
-  iIntros "Hwp".
-  rewrite iter_unfold.
-  iApply wp_bind.
-  iApply (wp_mono with "Hwp").
-  iIntros ([a | b]) "H /=".
-  - by iApply wp_think.
-  - by iApply wp_return.
-Qed.
+Admitted.
+
+Lemma step_thread_adequacy {R} (Φ Ψ: R -> iProp Σ) 
+  (h: heap nat)
+  (ts: list (thread nat R))
+  (ct: thread nat R):
+  wp_thread (state_interp γ) ct Ψ -∗
+  state_interp γ h -∗
+  ([∗ list] t ∈ ts, wp_thread (state_interp γ) t Φ) ==∗ ▷
+  match runState (step_thread ct) h ts with
+  | Here (ct', h', ts') => wp_thread (state_interp γ) ct' Ψ ∗ state_interp γ h'
+                          ∗ [∗ list] t ∈ ts', wp_thread (state_interp γ) t Φ
+  | ProgErr => False
+  | EvalErr => True
+  end.
+Proof.
+Admitted.
+(*
+Definition step_expr {V R A} (e: expr V A): state V R (expr V A) :=
+Definition step_thread {V R} (t: thread V R) : state V R (thread V R) :=
+Definition single_step_thread {V R} (s: scheduler V R): state V R (scheduler V R ) :=
+Fixpoint eval_threaded {V R} (n: nat) (s : scheduler V R) {struct n}: state V R R :=
+*)
+
+Lemma single_step_thread_adequacy {R} (Φ: R -> iProp Σ) 
+  (h: heap nat)
+  (s: scheduler nat R)
+  (ts: list (thread nat R)):
+  state_interp γ h -∗
+  ([∗ list] t ∈ ts, wp_thread (state_interp γ) t Φ) ==∗ ▷
+  match runState (single_step_thread s) h ts with
+  | Here (s', h', ts') => state_interp γ h'
+                          ∗ [∗ list] t ∈ ts', wp_thread (state_interp γ) t Φ
+  | ProgErr => False
+  | EvalErr => True
+  end.
+Proof.
+Admitted.
+
+Lemma eval_threaded_adequacy {R} (Φ: R -> iProp Σ) (n: nat)
+  (h: heap nat)
+  (s: scheduler nat R)
+  (ts: list (thread nat R)):
+  state_interp γ h -∗
+  ([∗ list] t ∈ ts, wp_thread (state_interp γ) t Φ) -∗ 
+  Nat.iter n (λ P : iPropI Σ, |==> ▷ P) $ |==>
+  match runState (eval_threaded n s) h ts with
+  | Here (x, h', ts') => Φ x ∗ state_interp γ h'
+                          ∗ [∗ list] t ∈ ts', wp_thread (state_interp γ) t Φ
+  | ProgErr => False
+  | EvalErr => True
+  end.
+Proof.
+Admitted.
+
+
+Lemma adequacy {R} (φ: R -> Prop) (n: nat) 
+  (SI: gmap nat nat -> iProp Σ)
+  (s: scheduler nat R)
+  (e: expr nat R)
+  (st st': heap nat)
+  : (∀ γ, ⊢ wp (state_interp γ) e (λ x, ⌜φ x⌝)) ->
+  match run_program n s e with
+  | Here x => φ x
+  | ProgErr => False
+  | EvalErr => True
+  end.
+  Proof.
+  Admitted.
+
+(* 
+
+
+
+
+  adequacy statement : voor alle schedelures alle initieele heaps.
+  - Als het interpret naar een value in een aantal stappen
+  - En er is een wp voor die expressie
+  - Dan krijgen we die pure post conditie er uit.
+  - En het programma loopt af.
+  - 
+*)
